TestDuration.dfy
@@ -90,6 +90,16 @@ module TestDuration {
   assert Duration.GetSeconds(d8) == 2;
   assert Duration.GetMilliseconds(d8) == 500;
  //dafny verify TestDuration.dfy
+
+assert Duration.StringIndexOf("PT9650H30M45.123S", 'T') == 1;
+assert Duration.StringIndexOf("PT9650H30M45.123S", 'H') == 6;
+assert Duration.StringIndexOf("PT9650H30M45.123S", 'M') == 9;
+//assert Duration.StringIndexOf("PT9650H30M45.123S", '.') == 11;
+//assert Duration.StringIndexOf("PT9650H30M45.123S", 'S') == 15;
+ var custom_string := Duration.ParseString("PT1H1M1");
+
+ assert Duration.GetMilliseconds(custom_string) == 0;
+ assert Duration.GetSeconds(custom_string) == 3661;
   }
 
 }
